good progress in defining the representation in F*, however the SMT performance seems bad

iocy/poset.fst
@@ -3,16 +3,7 @@ module Poset
 open FStar.Tactics
 open FStar.List.Tot.Base
 
-(** *** The set **)
-type id_typ = nat
-
-type elem (a:Type) = id_typ * a
-//| El : id:id_typ -> v:a -> elem a
-
-let el_id (x:elem 'a) : id_typ = fst x
-let el_v (x:elem 'a) : 'a = snd x
-
-let make_el (id:id_typ) (v:'a) : elem 'a = (id, v)
+(** *** Definition of a special type of set **)
 
 (** We need a set that allows the same value to appear multiple times and that allows
     us to distingusih between the appearances.
@@ -26,19 +17,29 @@ let make_el (id:id_typ) (v:'a) : elem 'a = (id, v)
 
     However, the offset is "reversed".
 **)
+type prop_set a = a -> Type0
 
-type base_set a = elem a -> Type0
-let (∈) (#a:Type) (el:elem a) (s:base_set a) = s el
-let (∉) (#a:Type) (el:elem a) (s:base_set a) = ~(el ∈ s)
+type uniq_val_id = nat
+type uniq_val (a:Type) = uniq_val_id * a
+let uid (x:uniq_val 'a) : uniq_val_id = fst x
+let uv  (x:uniq_val 'a) : 'a = snd x
+let make_uniq_val (id:uniq_val_id) (v:'a) : uniq_val 'a = (id, v)
 
-type set0 a (n:nat) = ofst:nat{ofst >= n} -> base_set a
+type _set a = prop_set (uniq_val a)
+let (∈) (#a:Type) (x:uniq_val a) (s:_set a) = s x
+let (∉) (#a:Type) (x:uniq_val a) (s:_set a) = ~(x ∈ s)
+
+type set0 a (n:nat) = ofst:nat{ofst >= n} -> _set a
 type set a (n:nat) = s:(set0 a n){
-  (forall ofst x. x ∈ s ofst ==> (ofst-n) < el_id x /\ el_id x <= ofst) /\
+  (forall ofst x. x ∈ s ofst ==> (ofst-n) < uid x /\ uid x <= ofst) /\
   // (forall ofst i. (ofst-n) < i /\ i <= ofst ==> (exists x. id x == i /\ x ∈ s ofst)) /\
-  (forall ofst x y. x ∈ s ofst /\ y ∈ s ofst /\ x =!= y ==> el_id x =!= el_id y)
+  (forall ofst x y. x ∈ s ofst /\ y ∈ s ofst /\ x =!= y ==> uid x =!= uid y)
 //  (forall ofst x y. x ∈ s ofst /\ y ∈ s ofst /\ id x == id y ==> x == y)
 }
 
+type set_elem (a:Type) (n:nat) =
+  ofst:nat{ofst >= n} -> uniq_val a
+  
 let empty_set_lemma (s:set 'a 0) : Lemma (forall ofst x. x ∉ s ofst) = ()
 
 let empty_set (#a:Type) : set a 0 = fun _ _ -> False
@@ -46,67 +47,66 @@ let empty_set (#a:Type) : set a 0 = fun _ _ -> False
 let eq_set (s1:set 'a 'n) (s2:set 'a 'm) : Type0 =
   'n == 'm /\ (forall ofst x. s1 ofst x <==> s2 ofst x)
 
-let return_set (#a:Type) (x:a) : set a 1 = fun ofst y -> make_el ofst x == y
+let return_set (#a:Type) (x:a) : set a 1 = fun ofst y -> make_uniq_val ofst x == y
 
 let add_set (#a:Type) (#n:nat) (s:set a n) (x:a) : set a (n+1) =
-  fun (ofst:nat{ofst >= n+1}) y -> make_el ofst x == y \/ y ∈ s (ofst-1)
+  fun (ofst:nat{ofst >= n+1}) y -> make_uniq_val ofst x == y \/ y ∈ s (ofst-1)
 let (⊕) #a #n = add_set #a #n
-
-type set_elem (a:Type) (n:nat) =
-  ofst:nat{ofst >= n} -> elem a
-
-(**
-let lemma_mem_add (#a:Type) (x:a) (#n:nat) (s:set a n) (ofst:nat{ofst >= n+1}) :
-  Lemma (make_el ofst x ∈ (s ⊕ x) ofst) [SMTPat (make_el ofst x ∈ (s ⊕ x) ofst)] = ()
-
-let lemma_mem_add2 (#a:Type) (x:a) (#n:nat) (s:set a n) (ofst:nat{ofst >= n+2}) (y:a) :
-  Lemma (make_el (ofst-1) x ∈ ((s ⊕ x) ⊕ y) ofst) [SMTPat (make_el (ofst-1) x ∈ ((s ⊕ x) ⊕ y) ofst)] = ()
-**)
-
-let __test_set1 : set int 4 = (((return_set 1) ⊕ 2) ⊕ 2) ⊕ 4
-let _ = assert (make_el 2 2 ∈ __test_set1 4 /\ make_el 3 2 ∈ __test_set1 4)
-
-[@expect_failure]
-let _ = assert (make_el 4 2 ∈ __test_set1 4)
-[@expect_failure]
-let _ = assert (make_el 1 2 ∈ __test_set1 4)
-let _ = assert (make_el 1 2 ∉ __test_set1 4)
-
-let __test_mem (s0:nat{s0 >= 4}) =
-  assert (exists (id1 id2:id_typ). make_el id1 2 ∈ __test_set1 s0 /\ id1 <= id2 /\ make_el id2 2 ∈ __test_set1 s0)
-
-let _ = assert (exists (id1 id2:id_typ). id1 <= id2 /\ 
-                      make_el id1 1 ∈ __test_set1 4 /\
-                      make_el (id1+1) 2 ∈ __test_set1 4 /\
-                      make_el id2 2 ∈ __test_set1 4 /\
-                      make_el (id2+1) 4 ∈ __test_set1 4)
-
-let union_set (#a:Type) (#n #m:nat) (s0:set a n) (s1:set a m) : set a (n+m) =
-  fun (ofst:nat{ofst >= n+m}) x -> x ∈ s0 (ofst-m) \/ x ∈ s1 ofst
-
-let lemma_mem_union_set_rhs (#a:Type) (x:a) (#n:nat) (s1:set a n) (#m:nat) (s2:set a m) (id:id_typ) (ofst:nat{ofst >= n+m}) :
-  Lemma (requires (ofst-m < id))
-        (ensures (make_el id x ∈ (s1 `union_set` s2) ofst) <==>
-                 (make_el id x ∈ s2 ofst))
-  [SMTPat (make_el id x ∈ (s1 `union_set` s2) ofst)] = ()
-  
-let lemma_mem_union_set_lhs (#a:Type) (x:a) (#n:nat) (s1:set a n) (#m:nat) (s2:set a m) (id:id_typ) (ofst:nat{ofst >= n+m}) :
-  Lemma (requires (id <= ofst-m))
-        (ensures (make_el id x ∈ (s1 `union_set` s2) ofst) <==> 
-                (make_el id x ∈ s1 (ofst-m)))
-  [SMTPat (make_el id x ∈ (s1 `union_set` s2) ofst)] = ()
 
 let subset_set (#a:Type) (#n #m:nat) (s0:set a n) (s1:set a m) : Type0 =
   n <= m ==> (forall x (ofst:nat{ofst >= m}). x ∈ s0 ofst ==> x ∈ s1 ofst)
 let (⊆) #a #n #m = subset_set #a #n #m
 
+let union_set (#a:Type) (#n #m:nat) (s0:set a n) (s1:set a m) : set a (n+m) =
+  fun (ofst:nat{ofst >= n+m}) x -> x ∈ s0 (ofst-m) \/ x ∈ s1 ofst
+
+(**
+let lemma_mem_add (#a:Type) (x:a) (#n:nat) (s:set a n) (ofst:nat{ofst >= n+1}) :
+  Lemma (make_uniq_val ofst x ∈ (s ⊕ x) ofst) [SMTPat (make_uniq_val ofst x ∈ (s ⊕ x) ofst)] = ()
+
+let lemma_mem_add2 (#a:Type) (x:a) (#n:nat) (s:set a n) (ofst:nat{ofst >= n+2}) (y:a) :
+  Lemma (make_uniq_val (ofst-1) x ∈ ((s ⊕ x) ⊕ y) ofst) [SMTPat (make_uniq_val (ofst-1) x ∈ ((s ⊕ x) ⊕ y) ofst)] = ()
+**)
+
+let lemma_mem_union_set_rhs (#a:Type) (x:a) (#n:nat) (s1:set a n) (#m:nat) (s2:set a m) (id:uniq_val_id) (ofst:nat{ofst >= n+m}) :
+  Lemma (requires (ofst-m < id))
+        (ensures (make_uniq_val id x ∈ (s1 `union_set` s2) ofst) <==>
+                 (make_uniq_val id x ∈ s2 ofst))
+  [SMTPat (make_uniq_val id x ∈ (s1 `union_set` s2) ofst)] = ()
+  
+let lemma_mem_union_set_lhs (#a:Type) (x:a) (#n:nat) (s1:set a n) (#m:nat) (s2:set a m) (id:uniq_val_id) (ofst:nat{ofst >= n+m}) :
+  Lemma (requires (id <= ofst-m))
+        (ensures (make_uniq_val id x ∈ (s1 `union_set` s2) ofst) <==> 
+                (make_uniq_val id x ∈ s1 (ofst-m)))
+  [SMTPat (make_uniq_val id x ∈ (s1 `union_set` s2) ofst)] = ()
+
+let __test_set1 : set int 4 = (((return_set 1) ⊕ 2) ⊕ 2) ⊕ 4
+let _ = assert (make_uniq_val 2 2 ∈ __test_set1 4 /\ make_uniq_val 3 2 ∈ __test_set1 4)
+
+[@expect_failure]
+let _ = assert (make_uniq_val 4 2 ∈ __test_set1 4)
+[@expect_failure]
+let _ = assert (make_uniq_val 1 2 ∈ __test_set1 4)
+let _ = assert (make_uniq_val 1 2 ∉ __test_set1 4)
+
+let __test_mem (s0:nat{s0 >= 4}) =
+  assert (exists (id1 id2:uniq_val_id). make_uniq_val id1 2 ∈ __test_set1 s0 /\ id1 <= id2 /\ make_uniq_val id2 2 ∈ __test_set1 s0)
+
+let _ = assert (exists (id1 id2:uniq_val_id). id1 <= id2 /\ 
+                      make_uniq_val id1 1 ∈ __test_set1 4 /\
+                      make_uniq_val (id1+1) 2 ∈ __test_set1 4 /\
+                      make_uniq_val id2 2 ∈ __test_set1 4 /\
+                      make_uniq_val (id2+1) 4 ∈ __test_set1 4)
+
 let _ = assert (__test_set1 `subset_set` __test_set1)
 let __test_set2 = __test_set1 `union_set` __test_set1
 let _ = assert (__test_set1 `subset_set` __test_set2)
-let _ = assert (forall id v. make_el id v ∈ __test_set1 4 <==>
-                      make_el id v ∈ __test_set2 8 /\ make_el (id+4) v ∈ __test_set2 8)
+let _ = assert (forall id v. make_uniq_val id v ∈ __test_set1 4 <==>
+                      make_uniq_val id v ∈ __test_set2 8 /\ make_uniq_val (id+4) v ∈ __test_set2 8)
 
-type relation a (n:nat) = ofst:nat{ofst >= n} -> elem a -> elem a -> Type0
+(** *** Relation **)
+
+type relation a (n:nat) = ofst:nat{ofst >= n} -> uniq_val a -> uniq_val a -> Type0
 
 let empty_rel (#a:Type) (#n:nat) (s:set a n) : relation a n =
   fun ofst x y -> x ∈ s ofst /\ x == y
@@ -122,149 +122,286 @@ let extend_rel
   fun ofst ev1' ev2' -> ev1' ∈ s ofst /\ ev2' ∈ s ofst /\ 
     (((ev2 ofst `po ofst` ev1 ofst ==> ev1 ofst == ev2 ofst) /\ (ev1' `po ofst` ev1 ofst /\ ev2 ofst `po ofst` ev2')) \/ (ev1' `po ofst` ev2'))
 
+(** *** Data structure **)
+type th_id : eqtype = int
+type event a = option a
+type elem0 (a:Type) = th_id * event a
+type elem (a:Type) (n:nat) = set_elem (elem0 a) n
+
+let get_id (x:elem 'a 'n) (ofst:nat{ofst >= 'n}) : th_id = fst (snd (x ofst))
+
+let make_elem (#a:Type) (v:elem0 a) (n:nat) : elem a n = fun ofst -> make_uniq_val ofst v
+
 type poset0 (a:Type) (n:nat) =
-  set a n                (** set **)
+  set (elem0 a) n        (** set **)
   *
-  relation a n           (** partial order between elements **) 
+  relation (elem0 a) n   (** partial order between elements **) 
   *
-  option (set_elem a n)  (** the least element **)
+  option (elem a n)  (** the least element **)
   *
-  option (set_elem a n)  (** the maximal element of the main thread **)
+  (th_id -> option (elem a n)) (** the maximal elements, one for each thread not awaited **)
+  *
+  list (th_id * (elem a n))
 
 type poset (a:Type) (n:nat) =
   p:(poset0 a n){
-    let (s, rel, least, max_r) = p in
+    let (s, rel, least, maxs, urel) = p in
+
+    (** poset properties **)
     (forall ofst x. x ∈ s ofst ==> x `rel ofst` x) /\
     (forall ofst x y z. x ∈ s ofst /\ y ∈ s ofst /\ z ∈ s ofst ==> (x `rel ofst` y /\ y `rel ofst` z ==> x `rel ofst` z)) /\
     (forall ofst x y. x ∈ s ofst /\ y ∈ s ofst ==> (x `rel ofst` y /\ y `rel ofst` x ==> x == y)) /\
+
+    (** property of the least element **)
     (None? least <==> n == 0) /\
-    (Some? least ==> (forall ofst. Some?.v least ofst ∈ s ofst /\ (forall x. x ∈ s ofst ==> Some?.v least ofst `rel ofst` x))) /\
-    (None? max_r <==> n == 0) /\
-    (Some? max_r ==> (forall ofst. Some?.v max_r ofst ∈ s ofst)) // /\ (forall x. x ∈ s ofst /\ x =!= Some?.v max_r ofst ==> ~(Some?.v max_r ofst `rel ofst` x))))
-  }
+    (n <> 0 ==> Some? least /\ (forall ofst. Some?.v least ofst ∈ s ofst /\ (forall x. x ∈ s ofst ==> Some?.v least ofst `rel ofst` x))) /\
 
-let empty_poset (#a:Type) : poset a 0 = (empty_set, empty_rel empty_set, None, None)
+    (** each element of the maxs function is a maximal element **)
+    (forall (tid:th_id). match maxs tid with
+      | Some max -> (forall ofst. tid == get_id max ofst /\ max ofst ∈ s ofst)
+      | _ -> True) /\
 
-let return_poset (el:'e) : poset 'e 1 =
-  let s = return_set el in
-  (s, empty_rel s, Some (fun ofst -> make_el ofst el), Some (fun ofst -> make_el ofst el))
+    (** the maxs function captures all maximal elements **)
+    (forall (x:elem a n) ofst. (x ofst ∈ s ofst /\ (forall (y:elem a n). y ofst ∈ s ofst /\ get_id x ofst == get_id y ofst ==> ~(x ofst `rel ofst` y ofst))) ==>
+      (maxs (get_id x ofst) == Some x)) /\
+
+    (n <> 0 ==> (forall ofst. Some? (maxs (get_id (Some?.v least) ofst)))) /\
+
+    (** urel properties **)
+    (forall tid x. (tid, x) `memP` urel ==> (None? (maxs tid)) /\ (forall ofst. x ofst ∈ s ofst))
+}
+
+let empty_poset (#a:Type) : poset a 0 = (empty_set, empty_rel empty_set, None, (fun _ -> None), [])
+
+let return_poset (el0:elem0 'a) : poset 'a 1 =
+  let s = return_set el0 in
+  let el = make_elem el0 1 in
+  let maxs = (fun tid -> if tid = (fst el0) then Some el else None) in
+  (s, empty_rel s, Some el, maxs, [])
 
 let new_po
   (#n #m:nat)
-  (s1:set 'e n)
-  (rel1:relation 'e n)
-  (s2:set 'e m)
-  (rel2:relation 'e m)
-  (max_r1 : (ofst:nat{ofst >= n}) -> elem 'e)
-  : relation 'e (n+m) = (fun (ofst:nat{ofst >= n + m}) x y ->
-  (x ∈ s1 (ofst-m) /\ y ∈ s1 (ofst-m) /\ x `rel1 (ofst-m)` y) \/
-  (x ∈ s2 ofst /\ y ∈ s2 ofst /\ x `rel2 ofst` y) \/
-  (x ∈ s1 (ofst-m) /\ y ∈ s2 ofst /\ x `rel1 (ofst-m)` (max_r1 (ofst-m))))
+  (s1:set (elem0 'e) n)
+  (rel1:relation (elem0 'e) n)
+  (s2:set (elem0 'e) m)
+  (rel2:relation (elem0 'e) m)
+  (least1 : option (elem 'e n))
+  (maxs1 : th_id -> option (elem 'e n))
+  (urel2 : list (th_id * elem 'e m))
+  (_:squash (n <> 0 ==> (forall (ofst:nat{ofst >= n+m}). Some? least1 /\ Some? (maxs1 (get_id (Some?.v least1) (ofst-m))))))
+  : relation (elem0 'e) (n+m) = (
+  fun (ofst:nat{ofst >= n + m}) x y ->
+    (x ∈ s1 (ofst-m) /\ y ∈ s1 (ofst-m) /\ x `rel1 (ofst-m)` y) \/
+    (x ∈ s2 ofst /\ y ∈ s2 ofst /\ x `rel2 ofst` y) \/
+    (x ∈ s1 (ofst-m) /\ y ∈ s2 ofst /\ x `rel1 (ofst-m)` (Some?.v (maxs1 (get_id (Some?.v least1) (ofst-m)))) (ofst-m)) \/
+    (x ∈ s1 (ofst-m) /\ y ∈ s2 ofst /\ (exists (u:th_id * elem 'e m). u `memP` urel2 /\ Some? (maxs1 (fst u)) /\
+                                             x `rel1 (ofst-m)` (Some?.v (maxs1 (fst u)) (ofst-m)) /\ snd u ofst `rel2 ofst` y))
+  )
 
-let append_poset (#n #m:nat) (pos1:poset 'e n) (pos2:poset 'e m) : poset 'e (n+m) =
-  let (s1, rel1, least1, max_r1)  = pos1 in
-  let (s2, rel2, least2, max_r2) = pos2 in
+let new_maxs 
+  (#n #m:nat)
+  (maxs1 : th_id -> option (elem 'e n))
+  (maxs2 : th_id -> option (elem 'e m))
+  : th_id -> option (elem 'e (n+m)) = 
+  (fun tid -> 
+    match maxs2 tid with
+    | Some x -> Some (fun (ofst:nat{ofst >= n+m}) -> x ofst)
+    | None -> begin
+           match maxs1 tid with
+           | None -> None
+           | Some x -> Some (fun (ofst:nat{ofst >= n+m}) -> x (ofst-m))
+    end)
+
+let new_urel
+  (#n #m:nat)
+  (maxs1 : th_id -> option (elem 'e n))
+  (urel1 : list (th_id * elem 'e n))
+  (urel2 : list (th_id * elem 'e m))
+  : list (th_id * elem 'e (n+m)) =
+  List.Tot.filter (fun (tid,_) -> not (Some? (maxs1 tid))) (
+    (List.Tot.map #(th_id * elem 'e n) #(th_id * elem 'e (n+m)) (fun (tid, el) -> (tid, (fun (ofst:nat{ofst >= n+m}) -> el (ofst-m)))) urel1) @
+    (List.Tot.map #(th_id * elem 'e m) #(th_id * elem 'e (n+m)) (fun (tid, el) -> (tid, (fun (ofst:nat{ofst >= n+m}) -> el ofst))) urel2))
+
+let lemma_new_urel
+  (#n #m:nat)
+  (maxs1 : th_id -> option (elem 'e n))
+  (urel1 : list (th_id * elem 'e n))
+  (urel2 : list (th_id * elem 'e m))
+  (maxs : th_id -> option (elem 'e (n+m)))
+  (s : set (elem0 'e) (n+m)) :
+  Lemma (
+    let urel = new_urel maxs1 urel1 urel2 in
+    (forall tid x. (tid, x) `memP` urel ==> (None? (maxs tid)) /\ (forall ofst. x ofst ∈ s ofst))) = admit ()
+
+let concat_poset (#n #m:nat) (pos1:poset 'e n) (pos2:poset 'e m) : poset 'e (n+m) =
+  let (s1, rel1, least1, maxs1, urel1)  = pos1 in
+  let (s2, rel2, least2, maxs2, urel2) = pos2 in
   match least1, least2 with
   | None, None
-  | None, _ -> pos2
-  | _, None -> pos1
+  | None, _ -> assert (n+m == m); pos2
+  | _, None -> assert (n+m == n); pos1
   | _, _ -> begin
     let s = s1 `union_set` s2 in
-    let rel : relation 'e (n+m) = new_po s1 rel1 s2 rel2 (Some?.v max_r1) in
-    let least = Some (fun (ofst:nat{ofst >= n+m}) -> Some?.v least1 (ofst-m)) in
-    let max = Some (fun (ofst:nat{ofst >= n+m}) -> Some?.v max_r2 ofst) in
-    (s1 `union_set` s2, rel, least , max)
+    let rel : relation (elem0 'e) (n+m) = new_po s1 rel1 s2 rel2 least1 maxs1 urel2 () in
+    let least : option (elem 'e (n+m)) = Some (fun (ofst:nat{ofst >= n+m}) -> Some?.v least1 (ofst-m)) in
+    let maxs = new_maxs maxs1 maxs2 in
+    let urel = new_urel maxs1 urel1 urel2 in
+    let p : poset0 'e (n+m) = (s, rel, least, maxs, urel) in
+
+    assert (forall ofst x. x ∈ s ofst ==> x `rel ofst` x);
+    assert (forall ofst x y z. x ∈ s ofst /\ y ∈ s ofst /\ z ∈ s ofst ==> (x `rel ofst` y /\ y `rel ofst` z ==> x `rel ofst` z));
+    assert (forall ofst x y. x ∈ s ofst /\ y ∈ s ofst ==> (x `rel ofst` y /\ y `rel ofst` x ==> x == y));
+
+    (** property of the least element **)
+    assert (None? least <==> n == 0);
+    assert (n <> 0 ==> Some? least /\ (forall ofst. Some?.v least ofst ∈ s ofst /\ (forall x. x ∈ s ofst ==> Some?.v least ofst `rel ofst` x)));
+
+    (** the maxs function captures all maximal elements **)
+    assert (forall (x:elem 'e n) ofst. (x ofst ∈ s ofst /\ (forall (y:elem 'e n). y ofst ∈ s ofst /\ get_id x ofst == get_id y ofst ==> ~(x ofst `rel ofst` y ofst))) ==>
+      (maxs (get_id x ofst) == Some x));
+
+    assert (n <> 0 ==> (forall ofst. Some? (maxs (get_id (Some?.v least) ofst))));
+
+    (** the maxs function returns the last event produced by the thread `tid` **)
+    assert (forall (tid:th_id). match maxs tid with
+      | Some max -> (forall ofst. tid == get_id max ofst /\ max ofst ∈ s ofst)
+      | _ -> True);
+
+    lemma_new_urel maxs1 urel1 urel2 maxs s;
+    (** urel properties **)
+    assert (forall tid x. (tid, x) `memP` urel ==> (None? (maxs tid)) /\ (forall ofst. x ofst ∈ s ofst));
+    p
   end
 
 let subset_poset (#n #m:nat) (pos1:poset 'e n) (pos2:poset 'e m) : Type0 =
-  let (s1, rel1, least1, max_r1) = pos1 in
-  let (s2, rel2, least2, max_r2) = pos2 in
+  let (s1, rel1, least1, _, _) = pos1 in
+  let (s2, rel2, least2, _, _) = pos2 in
   s1 `subset_set` s2 /\
   (forall ofst x y. x ∈ s1 ofst /\ y ∈ s1 ofst /\ x `rel1 ofst` y ==> x `rel2 ofst` y)
 
-type event_typ 'e = option (nat * 'e)
-
-let op (e:'e) (th_id:nat) : poset (event_typ 'e) 1 =
-  let s = return_set (Some (th_id, e)) in
-  (s, empty_rel s, Some (fun ofst -> make_el ofst (Some (th_id, e))), Some (fun ofst -> make_el ofst (Some (th_id, e))))
-
+let op (tid:th_id) (e:'e) : poset 'e 1 =
+  return_poset (tid, Some e)
 
 (**
-     least ofst                               make_el (ofst-1) None        (new least) 
+     least ofst                               make_uniq_val (ofst-1) None        (new least) 
       |             async                   /        \
       |          ---------->               /          \
       |                                   v           v
-      v                              least (ofst-2)   make_el ofst None    (new max_r)
+      v                              least (ofst-2)   make_uniq_val ofst None    (new max_r)
      max_r ofst                            |
                                           |
                                           v
                                     max_r (ofst-2)
 **)
 
-let async (#n:nat) (p:poset (event_typ 'e) n) : poset (event_typ 'e) (n+2) = 
-  let (s, rel, least, max_r) = p in
-  let s' = s `union_set` (return_set None `union_set` return_set None) in
-  assert (forall ofst. make_el ofst None ∈ s' ofst /\ make_el (ofst-1) None ∈ s' ofst);
-  let rel' : relation (event_typ 'e) (n+2) = (fun ofst x y -> (x == make_el (ofst-1) None /\ y ∈ s' ofst) \/
-                                            (x == make_el ofst None /\ y == make_el ofst None) \/
-                                            (x ∈ s (ofst-2) /\ y ∈ s (ofst-2) /\ x `rel (ofst-2)` y)) in
-  (s', rel', Some (fun (ofst:nat{ofst >= n+2}) -> make_el (ofst-1) None), Some (fun ofst -> make_el ofst None))
+(** here tid is the id of the current thread, 
+    and p has a different id (aka get_id least <> tid) **)
+let async (#n:nat) (tid:th_id) (p:poset 'e n) :
+  Pure (poset 'e (n+1)) 
+    (requires (let (_, _, _, maxs, _) = p in None? (maxs tid)))
+    (ensures (fun _ -> True)) = 
+  let cp = return_poset (tid, None) in 
+  let (s, rel, least, maxs, urel) = p in
+  let urel' = if Some? least then (tid, Some?.v least)::urel else urel in
+  let p' : poset 'e n = (s, rel, least, maxs, urel') in
+  cp `concat_poset` p'
 
-(** CA: Not very principled since the po is defined over xs and ys which are not part of S **)
-let await (#e:Type) (th_id:nat) : poset (event_typ e) 1 =
-  let s : set (event_typ e) 1 = return_set None in
-  let rel = (fun ofst x y -> (x ∈ s ofst /\ y ∈ s ofst) \/ (y == make_el ofst None /\ Some? (el_v x) /\ fst (Some?.v (el_v x)) == th_id)) in
-  (s, rel, Some (fun ofst -> make_el ofst None), Some (fun ofst -> make_el ofst None))
+let await (#e:Type) (tid:th_id) (wid:th_id{wid <> tid}) : poset e 1 =
+  let (s, rel, least, maxs, urel) = return_poset (tid, None) in
+  (s, rel, least, maxs, [(wid, Some?.v least)])
 
-let prog04 () : poset (event_typ int) 5 = (op 1 1 `append_poset` async (op 2 2)) `append_poset` op 3 1
+(** *** Tests **)
+let prog01 () : poset int 3 = op 1 1 `concat_poset` (op 1 2 `concat_poset` op 1 3)
+
+#set-options "--timing"
+let __test_prog01 () = 
+  let (s, rel, least, maxs, urel) = prog01 () in
+  assert (Some? least /\ Some?.v least 3 == make_uniq_val 1 (1, Some 1));
+  assert (urel == []);
+  assert (forall tid. tid <> 1 ==> None? (maxs tid));
+  assert (Some? (maxs 1) /\ Some?.v (maxs 1) 3 == make_uniq_val 3 (1, Some 3));
+  assert (make_uniq_val 1 (1, Some 1) ∈ s 3);
+  assert (make_uniq_val 2 (1, Some 2) ∈ s 3);
+  assert (make_uniq_val 3 (1, Some 3) ∈ s 3);
+  assert (make_uniq_val 1 (1, Some 1) `rel 3` make_uniq_val 2 (1, Some 2));
+  assert (make_uniq_val 1 (1, Some 1) `rel 3` make_uniq_val 3 (1, Some 3));
+  assert (~(make_uniq_val 2 (1, Some 2) `rel 3` make_uniq_val 1 (1, Some 1)));
+  ()
+#reset-options
+
+let prog04 () : poset int 4 = (op 1 1 `concat_poset` async 1 (op 2 2)) `concat_poset` op 1 3
 
 #set-options "--timing"
 let __test_prog04 () = 
-  let (s, rel, least, max_r) = prog04 () in
-  assert (Some? least /\ Some?.v least 5 == make_el 1 (Some (1,1)));
-  assert (Some? max_r /\ Some?.v max_r 5 == make_el 5 (Some (1,3)));
-  assert (make_el 1 (Some (1,1)) ∈ s 5);
-  assert (make_el 2 (Some (2,2)) ∈ s 5);
-  assert (make_el 3 None ∈ s 5);
-  assert (make_el 4 None ∈ s 5);
-  assert (make_el 5 (Some (1,3)) ∈ s 5);
-  assert (make_el 1 (Some (1,1)) `rel 5` make_el 2 (Some (2,2)));
-  assert (~(make_el 5 (Some (1,3)) `rel 5` make_el 2 (Some (2,2))))
+  let (s, rel, least, maxs, urel) = prog04 () in
+  assert (Some? least /\ Some?.v least 4 == make_uniq_val 1 (1, Some 1));
+ // assert (Some? max_r /\ Some?.v maxs 4 == make_uniq_val 4 (Some (1,3)));
+  assert (make_uniq_val 1 (1, Some 1) ∈ s 4);
+  assert (make_uniq_val 2 (1, None) ∈ s 4);
+  assert (make_uniq_val 3 (2, Some 2) ∈ s 4);
+  assert (make_uniq_val 4 (1, Some 3) ∈ s 4);
+  assert (make_uniq_val 1 (1, Some 1) `rel 4` make_uniq_val 3 (2, Some 2));
+  assert (~(make_uniq_val 4 (1, Some 3) `rel 4` make_uniq_val 3 (2, (Some 2))));
+  ()
 #reset-options
   
-let prog05 () : poset (event_typ int) 4 = async (op 2 2) `append_poset` await 2
+let prog05 () : poset int 3 = async 1 (op 2 2) `concat_poset` await 1 2
 
 #set-options "--timing"
-let __test_prog05 () = 
-  let (s, rel, least, max_r) = prog05 () in
-  assert (Some? least /\ Some?.v least 4 == make_el 2 None);
-  assert (Some? max_r /\ Some?.v max_r 4 == make_el 4 None);
-  assert (make_el 1 (Some (2,2)) ∈ s 4);
-  assert (make_el 2 None ∈ s 4);
-  assert (make_el 3 None ∈ s 4);
-  assert (make_el 4 None ∈ s 4)
+let __test_prog05 () : Tot unit by (
+  norm [delta_only [`%async;`%await;`%op;`%concat_poset;`%return_poset;`%new_po];zeta;iota];
+  dump "H") = 
+  let (s, rel, least, maxs, urel) = async 1 (op 2 2) `concat_poset` await 1 2 in //prog05 () in
+  assert (Some? least /\ Some?.v least 3 == make_uniq_val 1 (1, None));
+  // assert (Some? max_r /\ Some?.v max_r 4 == make_uniq_val 4 None);
+  assert (make_uniq_val 1 (1, None) ∈ s 3);
+  assert (make_uniq_val 2 (2, Some 2) ∈ s 3);
+  assert (make_uniq_val 3 (1, None) ∈ s 3);
+  assert (make_uniq_val 2 (2, Some 2) `rel 3` make_uniq_val 3 (1, None));
+  assert (~(make_uniq_val 3 (1, None) `rel 3` make_uniq_val 2 (2, Some 2)));
+  ()
 #reset-options
+ 
+let lemma_mem_union_set_lhs' (#a:Type) (x:a) (id:uniq_val_id) (#n:nat) (s1:set a n) (#m:nat) (s2:set a m) (#r:nat) (s3:set a r) (ofst:nat{ofst >= n+m+r}) :
+  Lemma (requires (ofst-r-m < id /\ id <= ofst-r))
+        (ensures (make_uniq_val id x ∈ (s1 `union_set` (s2 `union_set` s3)) ofst) <==> 
+                 (make_uniq_val id x ∈ s2 (ofst-r)))
+  [SMTPat (make_uniq_val id x ∈ (s1 `union_set` (s2 `union_set` s3)) ofst)] = ()
+ 
+let lemma_mem_union_set_lhs'''' (#a:Type) (x:a) (id:uniq_val_id) (#n:nat) (s1:set a n) (#m:nat) (s2:set a m) (#r:nat) (s3:set a r) (ofst:nat{ofst >= n+m+r}) :
+  Lemma (requires (ofst-r < id))
+        (ensures (make_uniq_val id x ∈ (s1 `union_set` (s2 `union_set` s3)) ofst) <==> 
+                 (make_uniq_val id x ∈ s3 ofst))
+  [SMTPat (make_uniq_val id x ∈ (s1 `union_set` (s2 `union_set` s3)) ofst)] = ()
+ 
+let lemma_mem_union_set_lhs'' (#a:Type) (x:a) (id:uniq_val_id) (#n:nat) (s1:set a n) (#m:nat) (s2:set a m) (#r:nat) (s3:set a r) (ofst:nat{ofst >= n+m+r}) :
+  Lemma (requires (ofst-r-m < id /\ id <= ofst-r))
+        (ensures (make_uniq_val id x ∈ ((s1 `union_set` s2) `union_set` s3) ofst) <==> 
+                 (make_uniq_val id x ∈ s2 (ofst-r)))
+  [SMTPat (make_uniq_val id x ∈ ((s1 `union_set` s2) `union_set` s3) ofst)] = ()
+ 
+let lemma_mem_union_set_lhs''' (#a:Type) (x:a) (id:uniq_val_id) (#n:nat) (s1:set a n) (#m:nat) (s2:set a m) (#r:nat) (s3:set a r) (ofst:nat{ofst >= n+m+r}) :
+  Lemma (requires (id <= ofst-r-m))
+        (ensures (make_uniq_val id x ∈ ((s1 `union_set` s2) `union_set` s3) ofst) <==> 
+                 (make_uniq_val id x ∈ s1 (ofst-r-m)))
+  [SMTPat (make_uniq_val id x ∈ ((s1 `union_set` s2) `union_set` s3) ofst)] = ()
 
-let __test_prog05' () = 
-  let (s, rel, least, max_r) = prog05 () in
-  assert (~(make_el 1 (Some (2,2)) `rel 4` make_el 4 None))
+#set-options "--timing --z3rlimit 24"
 
 (** Test:
           (1,1)
             |
             *
            /  \
-       (2,2)   *
-         |     |
-         |   (1,3)
-           \   |
+      (2,2)    (1,3)
+            \  |
                *
                |
              (1,4)
 **)
 
-let prog1 : poset (event_typ int) 7 =
-  (((op 1 1 `append_poset` async (op 2 2)) `append_poset` (op 3 1)) `append_poset` await 2) `append_poset` op 4 1
+let prog1 : poset int 6 =
+  (((op 1 1 `concat_poset` async 1 (op 2 2)) `concat_poset` (op 1 3)) `concat_poset` await 1 2) `concat_poset` op 1 4
 
 // TODO: why do I have performance problems here?
 // TODO: test on a smaller case if await works:
@@ -274,62 +411,32 @@ let prog1 : poset (event_typ int) 7 =
 
 
 let __test_prog1' () = 
-  let (s, po, least, max_r) = prog1 in
-  assert (make_el 1 (Some (1,1)) ∈ s 7)
- 
-let lemma_mem_union_set_lhs' (#a:Type) (x:a) (id:id_typ) (#n:nat) (s1:set a n) (#m:nat) (s2:set a m) (#r:nat) (s3:set a r) (ofst:nat{ofst >= n+m+r}) :
-  Lemma (requires (ofst-r-m < id /\ id <= ofst-r))
-        (ensures (make_el id x ∈ (s1 `union_set` (s2 `union_set` s3)) ofst) <==> 
-                 (make_el id x ∈ s2 (ofst-r)))
-  [SMTPat (make_el id x ∈ (s1 `union_set` (s2 `union_set` s3)) ofst)] = ()
- 
-let lemma_mem_union_set_lhs'''' (#a:Type) (x:a) (id:id_typ) (#n:nat) (s1:set a n) (#m:nat) (s2:set a m) (#r:nat) (s3:set a r) (ofst:nat{ofst >= n+m+r}) :
-  Lemma (requires (ofst-r < id))
-        (ensures (make_el id x ∈ (s1 `union_set` (s2 `union_set` s3)) ofst) <==> 
-                 (make_el id x ∈ s3 ofst))
-  [SMTPat (make_el id x ∈ (s1 `union_set` (s2 `union_set` s3)) ofst)] = ()
- 
-let lemma_mem_union_set_lhs'' (#a:Type) (x:a) (id:id_typ) (#n:nat) (s1:set a n) (#m:nat) (s2:set a m) (#r:nat) (s3:set a r) (ofst:nat{ofst >= n+m+r}) :
-  Lemma (requires (ofst-r-m < id /\ id <= ofst-r))
-        (ensures (make_el id x ∈ ((s1 `union_set` s2) `union_set` s3) ofst) <==> 
-                 (make_el id x ∈ s2 (ofst-r)))
-  [SMTPat (make_el id x ∈ ((s1 `union_set` s2) `union_set` s3) ofst)] = ()
- 
-let lemma_mem_union_set_lhs''' (#a:Type) (x:a) (id:id_typ) (#n:nat) (s1:set a n) (#m:nat) (s2:set a m) (#r:nat) (s3:set a r) (ofst:nat{ofst >= n+m+r}) :
-  Lemma (requires (id <= ofst-r-m))
-        (ensures (make_el id x ∈ ((s1 `union_set` s2) `union_set` s3) ofst) <==> 
-                 (make_el id x ∈ s1 (ofst-r-m)))
-  [SMTPat (make_el id x ∈ ((s1 `union_set` s2) `union_set` s3) ofst)] = ()
-
-#set-options "--timing --z3rlimit 24"
+  let (s, rel, least, maxs, urel) = prog1 in
+  assert (make_uniq_val 1 (1, Some 1) ∈ s 6)
 
 let _ = 
-  let (s, po, least, max_r) = prog1 in
-  assert (make_el 1 (Some (1,1)) ∈ s 7)
+  let (s, rel, least, maxs, urel) = prog1 in
+  assert (make_uniq_val 1 (1, Some 1) ∈ s 6)
 
 let _ = 
-  let (s, po, least, max_r) = prog1 in
-  assert (make_el 2 (Some (2,2)) ∈ s 7)
+  let (s, rel, least, maxs, urel) = prog1 in
+  assert (make_uniq_val 2 (1, None) ∈ s 6)
 
 let _ = 
-  let (s, po, least, max_r) = prog1 in
-  assert (make_el 3 None ∈ s 7)
+  let (s, rel, least, maxs, urel) = prog1 in
+  assert (make_uniq_val 3 (2, Some 2) ∈ s 6)
 
 let _ = 
-  let (s, po, least, max_r) = prog1 in
-  assert (make_el 4 None ∈ s 7)
+  let (s, rel, least, maxs, urel) = prog1 in
+  assert (make_uniq_val 4 (1, Some 3) ∈ s 6)
 
 let _ = 
-  let (s, po, least, max_r) = prog1 in
-  assert (make_el 5 (Some (1,3)) ∈ s 7)
+  let (s, rel, least, maxs, urel) = prog1 in
+  assert (make_uniq_val 5 (1, None) ∈ s 6)
 
 let _ = 
-  let (s, po, least, max_r) = prog1 in
-  assert (make_el 6 None ∈ s 7)
-
-let _ = 
-  let (s, po, least, max_r) = prog1 in
-  assert (make_el 7 (Some (1,4)) ∈ s 7)
+  let (s, rel, least, maxs, urel) = prog1 in
+  assert (make_uniq_val 6 (1, Some 4) ∈ s 6)
   
 type trace 'e = list 'e
   
@@ -339,32 +446,36 @@ let empty_marked (#a:Type) : marked a = fun _ -> False
 
 let mark (m:marked 'a) (v:'a) : marked 'a = fun v' -> v == v' \/ m v'
 
-let rec sat0 (t:trace 'e) (#n:nat) (s:set (event_typ 'e) n) (rel:relation (event_typ 'e) n) (el_prev:elem (event_typ 'e)) (used_els:marked (elem (event_typ 'e))) : Type0 =
+let rec sat0 (t:trace 'e) (#n:nat) (s:set (elem0 'e) n) (rel:relation (elem0 'e) n)
+  (el_prev:uniq_val (elem0 'e)) (used_els:marked (uniq_val (elem0 'e))) : Type0 =
   match t with
   | [] -> True
   | ev :: tl -> exists el. 
                       (~(used_els el) /\
                       (el ∈ s n /\
                       (((el_prev `rel n` el) \/ ~(el `rel n` el_prev)) /\
-                      ((Some? (el_v el) /\ snd (Some?.v (el_v el)) == ev) /\
+                      ((Some? (snd (uv el)) /\ (Some?.v (snd (uv el))) == ev) /\
                       sat0 tl s rel el (mark used_els el)))))
 
-let sat (t:trace 'e) (#n:nat) (p:poset (event_typ 'e) n) : Type0 =
-  let (s, rel, least, _) = p in
+let sat (t:trace 'e) (#n:nat) (p:poset 'e n) : Type0 =
+  let (s, rel, least, maxs, urel) = p in
   match t with
   | [] -> n == 0
   | h :: tl -> Some? least /\ (let least_el = Some?.v least n in
-              match el_v least_el with
+              match snd (uv least_el) with
               | None -> sat0 t s rel least_el (mark empty_marked least_el)
-              | Some b' -> h == snd b' /\ sat0 tl s rel least_el (mark empty_marked least_el))
+              | Some b' -> h == b' /\ sat0 tl s rel least_el (mark empty_marked least_el))
 
 #set-options "--z3rlimit 64"
+#set-options "--z3rlimit 512 --fuel 200 --ifuel 200"
+#push-options "--timing"
+
 let _ = assert ([1;4] `sat` prog1) 
 // 3000-4000ms when sat0 uses ∈
 
 let _ = assert (~([4;1] `sat` prog1))
 
-#set-options "--z3rlimit 128"
+//#set-options "--z3rlimit 128"
 let _ = assert ([1;2;3] `sat` prog1) 
 
 let _ = assert (([1;2;4] `sat` prog1))
@@ -384,9 +495,9 @@ let rec test_membership0 (t:trace int) (#n:nat) (p:poset int n) (el_prev:elem in
   | [] -> True
   | h :: tl -> exists id_h. ~(marked_ids id_h) /\ 
                       id_h <= n /\
-                      (make_el id_h h ∈ s n) /\
-                      ((el_prev `rel n` make_el id_h h) \/ ~(make_el id_h h `rel n` el_prev)) /\
-                      test_membership0 tl p (make_el id_h h) (mark marked_ids id_h)
+                      (make_uniq_val id_h h ∈ s n) /\
+                      ((el_prev `rel n` make_uniq_val id_h h) \/ ~(make_uniq_val id_h h `rel n` el_prev)) /\
+                      test_membership0 tl p (make_uniq_val id_h h) (mark marked_ids id_h)
 
 let test_membership (t:trace int) (#n:nat) (p:poset int n) : Type0 =
   let (_, _, least, _) = p in
@@ -401,11 +512,11 @@ let test_membership (t:trace int) (#n:nat) (p:poset int n) : Type0 =
 let __test_set : set int 3 = ((empty_set ⊕ 1) ⊕ 2) ⊕ 3
 let __test_po : relation int 3 =
   extend_rel __test_set
-    (extend_rel __test_set (empty_rel __test_set) (fun id -> make_el (id-2) 1) (fun id -> make_el (id-1) 2))
-    (fun id -> make_el (id-2) 1) (fun id -> make_el id 3)
+    (extend_rel __test_set (empty_rel __test_set) (fun id -> make_uniq_val (id-2) 1) (fun id -> make_uniq_val (id-1) 2))
+    (fun id -> make_uniq_val (id-2) 1) (fun id -> make_uniq_val id 3)
 
 let __test_poset : poset int 3 =
-  (__test_set, __test_po, Some (fun (ofst:nat{ofst >= 3}) -> make_el (ofst-2) 1), Some (fun id -> make_el id 3))
+  (__test_set, __test_po, Some (fun (ofst:nat{ofst >= 3}) -> make_uniq_val (ofst-2) 1), Some (fun id -> make_uniq_val id 3))
 
 let __test_123 () =
   assert ([1;2] `test_membership` __test_poset);
@@ -432,13 +543,13 @@ let __test_po3 : relation int 4 =
   extend_rel __test_set3
     (extend_rel __test_set3
         (extend_rel __test_set3
-        (extend_rel __test_set3 (empty_rel __test_set3) (fun id -> make_el (id-3) 1) (fun id -> make_el (id-2) 2))
-        (fun id -> make_el (id-3) 1) (fun id -> make_el (id-1) 3))
-      (fun id -> make_el (id-1) 3) (fun id -> make_el id 4))
-    (fun id -> make_el (id-2) 2) (fun id -> make_el id 4)
+        (extend_rel __test_set3 (empty_rel __test_set3) (fun id -> make_uniq_val (id-3) 1) (fun id -> make_uniq_val (id-2) 2))
+        (fun id -> make_uniq_val (id-3) 1) (fun id -> make_uniq_val (id-1) 3))
+      (fun id -> make_uniq_val (id-1) 3) (fun id -> make_uniq_val id 4))
+    (fun id -> make_uniq_val (id-2) 2) (fun id -> make_uniq_val id 4)
    
 let __test_poset3 : poset int 4 =
-  (__test_set3, __test_po3, Some (fun (ofst:nat{ofst >= 4}) -> make_el (ofst-3) 1), Some (fun id -> make_el id 4)) 
+  (__test_set3, __test_po3, Some (fun (ofst:nat{ofst >= 4}) -> make_uniq_val (ofst-3) 1), Some (fun id -> make_uniq_val id 4)) 
 
 let _ =
   assert ([1;2;3;4] `test_membership` __test_poset3)
